# Recurrence Relation Solutions (with \(T(1)=1\))

Assume that \(n\) is a power of 2, so we can write:

\[
n = 2^k \quad \text{where } k = \log_2 n
\]

---

## 1. \(T(n) = T(n/2) + 1\)

Unroll the recurrence:

\[
T(n) = T(n/2) + 1
\]
\[
= T(n/4) + 2
\]
\[
= \dots
\]
\[
= T(1) + k
\]

Since \(T(1)=1\) and \(k=\log_2 n\):

\[
T(n) = 1 + \log_2 n
\]

✅ Final Answer:

\[
\boxed{T(n) = 1 + \log_2 n}
\]

---

## 2. \(T(n) = 2T(n/2) + 1\)

Let \(n = 2^k\) and define:

\[
S(k) = T(2^k)
\]

Then:

\[
S(k) = 2S(k-1) + 1,\quad S(0)=1
\]

Unrolling:

\[
S(k) = 2^kS(0) + \sum_{i=0}^{k-1}2^i
\]

Since:

\[
\sum_{i=0}^{k-1}2^i = 2^k - 1
\]

So:

\[
S(k) = 2^k + (2^k - 1) = 2^{k+1} - 1
\]

Convert back using \(2^k=n\):

\[
T(n) = 2n - 1
\]

✅ Final Answer:

\[
\boxed{T(n) = 2n - 1}
\]

---

## 3. \(T(n) = 2T(n/2) + n\)

Again let \(S(k) = T(2^k)\):

\[
S(k) = 2S(k-1) + 2^k,\quad S(0)=1
\]

Unroll:

\[
S(k) = 2^kS(0) + \sum_{j=1}^{k}2^{k-j}\cdot 2^j
\]

Notice:

\[
2^{k-j}\cdot 2^j = 2^k
\]

So the sum becomes:

\[
k\cdot 2^k
\]

Thus:

\[
S(k) = 2^k + k2^k = (k+1)2^k
\]

Convert back:

\[
T(n) = n(\log_2 n + 1)
\]

✅ Final Answer:

\[
\boxed{T(n) = n(\log_2 n + 1)}
\]

---

## 4. \(T(n) = 4T(n/2) + 3\)

Let \(S(k)=T(2^k)\):

\[
S(k) = 4S(k-1) + 3,\quad S(0)=1
\]

Unroll:

\[
S(k) = 4^kS(0) + 3\sum_{i=0}^{k-1}4^i
\]

Geometric series:

\[
\sum_{i=0}^{k-1}4^i = \frac{4^k-1}{4-1}
\]

So:

\[
S(k) = 4^k + 3\cdot \frac{4^k-1}{3}
\]

\[
= 4^k + (4^k - 1)
\]

\[
= 2\cdot 4^k - 1
\]

Since:

\[
4^k = (2^k)^2 = n^2
\]

We get:

\[
T(n) = 2n^2 - 1
\]

✅ Final Answer:

\[
\boxed{T(n) = 2n^2 - 1}
\]

---

# Summary of Results

| Recurrence Relation | Closed Form Solution |
|---------------------|----------------------|
| \(T(n)=T(n/2)+1\) | \(1+\log_2 n\) |
| \(T(n)=2T(n/2)+1\) | \(2n-1\) |
| \(T(n)=2T(n/2)+n\) | \(n(\log_2 n+1)\) |
| \(T(n)=4T(n/2)+3\) | \(2n^2-1\) |

---
